leave one assume for seq0

lib/bv32_mm_lemmas.i.dfy
@@ -82,5 +82,60 @@ module bv32_mm_lemmas refines generic_mm_lemmas {
         && rsa_params_inv(rsa)
     }
 
+    datatype mm_vars = mm_vars_cons(
+        mm_frame_ptr: uint32, // writable
+        mma_frame_ptr: uint32, // writable
+        iter_a: iter_t,
+        iter_b: iter_t,
+        iter_c: iter_t, // writable
+        iter_n: iter_t
+    )
+
+    predicate mm_vars_inv(
+        vars: mm_vars,
+        mem: mem_t,
+        a_ptr: int, a_idx: nat,
+        n_ptr: int, n_idx: int,
+        c_ptr: int, c_idx: int,
+        b_ptr: int, b_idx: int,
+        rsa: rsa_params)
+    {
+        && valid_frame_ptr(mem, vars.mm_frame_ptr, 8)
+        && valid_frame_ptr(mem, vars.mma_frame_ptr, 12)
+
+        && mvar_iter_inv(mem, vars.iter_a, a_ptr, a_idx, NA)
+        && mvar_iter_inv(mem, vars.iter_c, c_ptr, c_idx, NA)
+        && mvar_iter_inv(mem, vars.iter_b, b_ptr, b_idx, NA)
+        && mvar_iter_inv(mem, vars.iter_n, n_ptr, n_idx, rsa.M)
+
+        && vars.iter_c.base_addr != vars.iter_a.base_addr
+        && vars.iter_c.base_addr != vars.iter_n.base_addr
+        && vars.iter_c.base_addr != vars.iter_b.base_addr
+        && vars.iter_c.base_addr != vars.mma_frame_ptr
+
+        && vars.mm_frame_ptr != vars.mma_frame_ptr
+        && vars.mm_frame_ptr != vars.iter_a.base_addr
+        && vars.mm_frame_ptr != vars.iter_b.base_addr
+        && vars.mm_frame_ptr != vars.iter_c.base_addr
+        && vars.mm_frame_ptr != vars.iter_n.base_addr
+
+        && vars.mma_frame_ptr != vars.iter_a.base_addr
+        && vars.mma_frame_ptr != vars.iter_n.base_addr
+        && vars.mma_frame_ptr != vars.iter_b.base_addr
+
+        && rsa_params_inv(rsa)
+    }
+
+    function to_mma_vars(vars: mm_vars, a_i: uint32): mma_vars
+    {
+        mma_vars(vars.mma_frame_ptr,
+            vars.iter_a, a_i, vars.iter_a.index,
+            vars.iter_b, vars.iter_c, vars.iter_n)
+    }
+
+    function seq_zero(i: nat): seq<uint32>
+    {
+        GBV.BVSEQ.SeqZero(NUM_WORDS)
+    }
 
 }
